test.v
@@ -8,3 +8,5 @@ Definition test_move_vec : move_vec q := fun p:Player => m.
 
 
 Definition test_move_function : move_function := fun (q:State) (p:Player) => m.
+
+  
